library/init/reserved_notation.lean
@@ -13,10 +13,8 @@ structure has_zero [class] (A : Type) := (zero : A)
 structure has_one  [class] (A : Type) := (one : A)
 structure has_add  [class] (A : Type) := (add : A → A → A)
 structure has_mul  [class] (A : Type) := (mul : A → A → A)
-structure has_inv  [class] (A : Type) := (inv : A → A)
 structure has_neg  [class] (A : Type) := (neg : A → A)
 structure has_sub  [class] (A : Type) := (sub : A → A → A)
-structure has_div  [class] (A : Type) := (div : A → A → A)
 structure has_dvd  [class] (A : Type) := (dvd : A → A → Prop)
 structure has_mod  [class] (A : Type) := (mod : A → A → A)
 structure has_le   [class] (A : Type) := (le : A → A → Prop)
@@ -27,13 +25,15 @@ definition one  {A : Type} [s : has_one A]  : A            := has_one.one A
 definition add  {A : Type} [s : has_add A]  : A → A → A    := has_add.add
 definition mul  {A : Type} [s : has_mul A]  : A → A → A    := has_mul.mul
 definition sub  {A : Type} [s : has_sub A]  : A → A → A    := has_sub.sub
-definition div  {A : Type} [s : has_div A]  : A → A → A    := has_div.div
 definition dvd  {A : Type} [s : has_dvd A]  : A → A → Prop := has_dvd.dvd
 definition mod  {A : Type} [s : has_mod A]  : A → A → A    := has_mod.mod
 definition neg  {A : Type} [s : has_neg A]  : A → A        := has_neg.neg
-definition inv  {A : Type} [s : has_inv A]  : A → A        := has_inv.inv
 definition le   {A : Type} [s : has_le A]   : A → A → Prop := has_le.le
 definition lt   {A : Type} [s : has_lt A]   : A → A → Prop := has_lt.lt
+
+structure has_inv [class] (A : Type) := (invertible : A → Prop) (inv : ∀ a, invertible a → A)
+definition invertible {A : Type} [s : has_inv A] : A → Prop := has_inv.invertible
+definition inv {A : Type} [s : has_inv A] : ∀ (a : A) {H : invertible a}, A := has_inv.inv
 
 definition ge [reducible] {A : Type} [s : has_le A] (a b : A) : Prop := le b a
 definition gt [reducible] {A : Type} [s : has_lt A] (a b : A) : Prop := lt b a
@@ -198,11 +198,13 @@ reserve infixr ` :: `:67
 infix +    := add
 infix *    := mul
 infix -    := sub
-infix /    := div
 infix ∣    := dvd
 infix %    := mod
 prefix -   := neg
 postfix ⁻¹ := inv
+
+--notation a / b := (a * b⁻¹)
+
 infix ≤    := le
 infix ≥    := ge
 infix <    := lt
@@ -211,7 +213,7 @@ infix >    := gt
 notation [parsing_only] x ` +[`:65 A:0 `] `:0 y:65 := @add A _ x y
 notation [parsing_only] x ` -[`:65 A:0 `] `:0 y:65 := @sub A _ x y
 notation [parsing_only] x ` *[`:70 A:0 `] `:0 y:70 := @mul A _ x y
-notation [parsing_only] x ` /[`:70 A:0 `] `:0 y:70 := @div A _ x y
+notation [parsing_only] x ` /[`:70 A:0 `] `:0 y:70 := @mul A _ x (@inv A _ y _)
 notation [parsing_only] x ` ∣[`:70 A:0 `] `:0 y:70 := @dvd A _ x y
 notation [parsing_only] x ` %[`:70 A:0 `] `:0 y:70 := @mod A _ x y
 notation [parsing_only] x ` ≤[`:50 A:0 `] `:0 y:50 := @le A _ x y
